### Определение
* ==Бином Ньютона== - $(a+b)^n =\sum_{k=0}^{n} C_{n}^{k}*a^{n-k}*b^k$ 

### Доказательство
	Метод математической индукции
>База n=1

$$a+b = C_{1}^0a^1+C_{1}^{1}b^1\implies a+b=a+b$$

>Индукционное предположение: верно для n, индукционный шаг n+1

$(a+b)^{n+1}=\sum_{k=0}^{n+1}C_{n+1}^k*a^{n+1-k}*b^k$ 
$(a+b)^{n+1}=(a+b)(a+b)^n=(a+b)*(\sum_{k=0}^{n}C_{n}^{k}*a^{n-k}*b^k = (a+b)(C_{n}^0a^n+C_{n}^{1}a^{n-1}*b+\dots+C_{n}^{n-1}*a*b^{n-1}+C_{n}^{n}b^n)$
$C_{n}^0a^{n+1}+C_{n}^{1}a^{n}*b+\dots+C_{n}^{n-1}*a^{2}*b^{n-1}+C_{n}^{n}a*b^{n+1}+C_{n}^0a^n*b+C_{n}^{1}a^{n-1}*b^2+\dots+C_{n}^{n-1}*a*b^{n}+C_{n}^{n}b^{n+1}$
$C_{n}^{0}a^{n+1}+a^nb(C_{n}^1+C_{n}^0)+\dots+ab^n(C_{n}^n+C_{n}^{n-1})+C_{n}^n*b^{n+1}$

>$C_{n}^{k}+C_{n}^{k+1} = C_{n+1}^{k+1}$

$C_{n}^0a^{n+1}+a^nb*C_{n+1}^1+\dots+ab^n*C_{n+1}^n+C_{n}^nb^{n+1}$

>$C_{n}^0=C_{n}^n=1$

$\sum_{k=0}^{n+1}C_{n+1}^{k}*a^{n+1-k}*b^k$ ч.т.д